# Projection


## Definitions

### Distance between point and set

The distance $d$ from point $\mathbf{y} \in \mathbb{R}^n$ to closed set
$S \subset \mathbb{R}^n$:

$$
d(\mathbf{y}, S, \| \cdot \|) = \inf\{\|x - y\| \mid x \in S \}
$$

### Projection of a point on set

Projection of a point $\mathbf{y} \in \mathbb{R}^n$ on set
$S \subseteq \mathbb{R}^n$ is a point $\pi_S(\mathbf{y}) \in S$:

$$
\| \pi_S(\mathbf{y}) - \mathbf{y}\| \le \|\mathbf{x} - \mathbf{y}\|, \forall \mathbf{x} \in S
$$

- if a set is open, and a point is beyond this set, then its projection
  on this set does not exist.

- if a point is in set, then its projection is the point itself

- $$
  \pi_S(\mathbf{y}) = \underset{\mathbf{x}}{\operatorname{argmin}} \|\mathbf{x}-\mathbf{y}\|
  $$

- Let $S \subseteq \mathbb{R}^n$ - convex closed set. Let the point
  $\mathbf{y} \in \mathbb{R}^n$ и $\mathbf{\pi} \in S$. Then if for all
  $\mathbf{x} \in S$ the inequality holds:

  $$
    \langle \pi  -\mathbf{y}, \mathbf{x} - \pi\rangle \ge 0, 
    $$

  then $\pi$ is the projection of the point $\mathbf{y}$ on $S$, so
  $\pi_S (\mathbf{y}) = \pi$.

- Let $S \subseteq \mathbb{R}^n$ - affine set. Let we have points
  $\mathbf{y} \in \mathbb{R}^n$ and $\mathbf{\pi} \in S$. Then $\pi$ is
  a projection of point $\mathbf{y}$ on $S$, so
  $\pi_S (\mathbf{y}) = \pi$ if and only if for all $\mathbf{x} \in S$
  the inequality holds:

$$
\langle \pi  -\mathbf{y}, \mathbf{x} - \pi\rangle = 0 
$$

- **Sufficient conditions of existence of a projection**. If
  $S \subseteq \mathbb{R}^n$ - closed set, then the projection on set
  $S$ exists for any point.
- **Sufficient conditions of uniqueness of a projection**. If
  $S \subseteq \mathbb{R}^n$ - closed convex set, then the projection on
  set $S$ is unique for any point.

> [!EXAMPLE]
>
> ### Example
>
> <div>
>
> <div class="callout-example">
>
> Find $\pi_S (y) = \pi$, if
> $S = \{x \in \mathbb{R}^n \mid \|x - x_0\| \le R \}$, $y \notin S$
>
> > [!SOLUTION]
> >
> > ### Solution
> >
> > <div>
> >
> > <div class="callout-solution" collapse="true">
> >
> > <div id="fig-projection_ball">
> >
> > ![](proj_ball.svg)
> >
> > Figure 1: Projection of point to the ball
> >
> > </div>
> >
> > - Build a hypothesis from the figure:
> >   $\pi = x_0 + R \cdot \frac{y - x_0}{\|y - x_0\|}$
> >
> > - Check the inequality for a convex closed set:
> >   $(\pi - y)^T(x - \pi) \ge 0$
> >
> >   $$
> >     \left( x_0 - y + R \frac{y - x_0}{\|y - x_0\|} \right)^T\left( x - x_0 - R \frac{y - x_0}{\|y - x_0\|} \right) =
> >     $$
> >
> >   $$
> >     \left( \frac{(y - x_0)(R - \|y - x_0\|)}{\|y - x_0\|} \right)^T\left( \frac{(x-x_0)\|y-x_0\|-R(y - x_0)}{\|y - x_0\|} \right) =
> >     $$
> >
> >   $$
> >     \frac{R - \|y - x_0\|}{\|y - x_0\|^2} \left(y - x_0 \right)^T\left( \left(x-x_0\right)\|y-x_0\|-R\left(y - x_0\right) \right) = 
> >     $$
> >
> >   $$
> >     \frac{R - \|y - x_0\|}{\|y - x_0\|} \left( \left(y - x_0 \right)^T\left( x-x_0\right)-R\|y - x_0\| \right) =
> >     $$
> >
> >   $$
> >     \left(R - \|y - x_0\| \right) \left( \frac{(y - x_0 )^T( x-x_0)}{\|y - x_0\|}-R \right)
> >     $$
> >
> > - The first factor is negative for point selection $y$. The second
> >   factor is also negative, which follows from the Cauchy-Bunyakovsky
> >   inequality:
> >
> >   $$
> >     (y - x_0 )^T( x-x_0) \le \|y - x_0\|\|x-x_0\|
> >     $$
> >
> >   $$
> >     \frac{(y - x_0 )^T( x-x_0)}{\|y - x_0\|} - R \le \frac{\|y - x_0\|\|x-x_0\|}{\|y - x_0\|} - R = \|x - x_0\| - R \le 0
> >     $$
> >
> > </div>
> >
> > </div>
>
> </div>
>
> </div>

> [!EXAMPLE]
>
> ### Example
>
> <div>
>
> <div class="callout-example">
>
> Find $\pi_S (y) = \pi$, if
> $S = \{x \in \mathbb{R}^n \mid c^T x = b \}$, $y \notin S$.
>
> > [!SOLUTION]
> >
> > ### Solution
> >
> > <div>
> >
> > <div class="callout-solution" collapse="true">
> >
> > <div id="fig-projection_halfspace">
> >
> > ![](proj_half.svg)
> >
> > Figure 2: Projection of point to the halfspace
> >
> > </div>
> >
> > - Build a hypothesis from the figure: $\pi = y + \alpha c$.
> >   Coefficient $\alpha$ is chosen so that $\pi \in S$: $c^T \pi = b$,
> >   so:
> >
> >   $$
> >     c^T (y + \alpha c) = b
> >     $$
> >
> >   $$
> >     c^Ty + \alpha c^T c = b
> >     $$
> >
> >   $$
> >     c^Ty = b - \alpha c^T c
> >     $$
> >
> > - Check the inequality for a convex closed set:
> >   $(\pi - y)^T(x - \pi) \ge 0$
> >
> >   $$
> >     (y + \alpha c - y)^T(x - y - \alpha c) = 
> >     $$
> >
> >   $$
> >      \alpha c^T(x - y - \alpha c) = 
> >     $$
> >
> >   $$
> >      \alpha (c^Tx) - \alpha (c^T y) - \alpha^2 (c^Tc) = 
> >     $$
> >
> >   $$
> >      \alpha b - \alpha (b - \alpha c^T c) - \alpha^2 c^Tc = 
> >     $$
> >
> >   $$
> >      \alpha b - \alpha b + \alpha^2 c^T c - \alpha^2 c^Tc = 0 \ge 0
> >     $$
> >
> > </div>
> >
> > </div>
>
> </div>
>
> </div>

> [!EXAMPLE]
>
> ### Example
>
> <div>
>
> <div class="callout-example">
>
> Find $\pi_S (y) = \pi$, if
> $S = \{x \in \mathbb{R}^n \mid Ax = b, A \in \mathbb{R}^{m \times n},  b \in \mathbb{R}^{m} \}$,
> $y \notin S$.
>
> > [!SOLUTION]
> >
> > ### Solution
> >
> > <div>
> >
> > <div class="callout-solution" collapse="true">
> >
> > <div id="fig-projection_linear_system">
> >
> > ![](proj_poly.svg)
> >
> > Figure 3: Projection of point to the set of linear equations
> >
> > </div>
> >
> > - Build a hypothesis from the figure:
> >   $\pi = y + \sum\limits_{i=1}^m\alpha_i A_i = y + A^T \alpha$.
> >   Coefficient $\alpha$ is chosen so that $\pi \in S$: $A \pi = b$,
> >   so:
> >
> >   $$
> >     A(y + A^T\alpha) = b
> >     $$
> >
> >   $$
> >     Ay = b - A A^T\alpha
> >     $$
> >
> > - Check the inequality for a convex closed set:
> >   $(\pi - y)^T(x - \pi) \ge 0$
> >
> >   $$
> >     (y + A^T\alpha  - y)^T(x - y - A^T\alpha) = 
> >     $$
> >
> >   $$
> >      \alpha^T A(x - y - A^T\alpha) = 
> >     $$
> >
> >   $$
> >      \alpha^T (Ax) - \alpha^T (A y) - \alpha^T (AA^T \alpha) = 
> >     $$
> >
> >   $$
> >      \alpha^T b - \alpha^T (b - A A^T\alpha) - \alpha^T AA^T \alpha = 
> >     $$
> >
> >   $$
> >      \alpha^T b - \alpha^T b + \alpha^T AA^T \alpha - \alpha^T AA^T \alpha = 0 \ge 0
> >     $$
> >
> > </div>
> >
> > </div>
>
> </div>
>
> </div>
