# Conjugate set


## Conjugate (Fenchel conjugate, dual, Fenchel dual) set

### Definitions

Let $S \subseteq \mathbb{R}^n$ be an arbitrary non-empty set. Then its
conjugate set is defined as:

$$
S^* = \{y \in \mathbb{R}^n \mid \langle y, x\rangle \ge -1 \;\; \forall x \in S\}
$$

<div id="fig-conjugate_set">

![](conjugate_set.svg)

Figure 1: Convex sets may be described in a dual way - through the
elements of the set and through the set of hyperplanes supporting it

</div>

A set $S^{**}$ is called double conjugate to a set $S$ if:

$$
S^{**} = \{y \in \mathbb{R}^n \mid \langle y, x\rangle \ge -1 \;\; \forall x \in S^*\}
$$

- The sets $S_1$ and $S_2$ are called **inter-conjugate** if
  $S_1^* = S_2, S_2^* = S_1$.
- A set $S$ is called **self-conjugate** if $S^{*} = S$.

### Properties

- A conjugate set is always closed, convex, and contains zero.

- For an arbitrary set $S \subseteq \mathbb{R}^n$:

  $$
     S^{**} = \overline{ \mathbf{conv} (S \cup \{0\}) }
    $$

- If $S_1 \subseteq S_2$, then $S_2^* \subseteq S_1^*$.

- $\left( \bigcup\limits_{i=1}^m S_i \right)^* = \bigcap\limits_{i=1}^m S_i^*$.

- If $S$ is closed, convex, and includes $0$, then $S^{**} = S$.

- $S^* = \left(\overline{S}\right)^*$.

### Examples

> [!EXAMPLE]
>
> ### Example
>
> <div>
>
> <div class="callout-example">
>
> Prove that $S^* = \left(\overline{S}\right)^*$.
>
> > [!SOLUTION]
> >
> > ### Solution
> >
> > <div>
> >
> > <div class="callout-solution" collapse="true">
> >
> > - $S \subset \overline{S}\rightarrow \left(\overline{S}\right)^* \subset S^*$.
> > - Let $p \in S^*$ and
> >   $x_0 \in \overline{S}, x_0 = \underset{k \to \infty}{\operatorname{lim}} x_k$.
> >   Then by virtue of the continuity of the function $f(x) = p^Tx$, we
> >   have: $p^T x_k \ge -1 \to p^Tx_0 \ge -1$. So
> >   $p \in \left(\overline{S}\right)^*$, hence
> >   $S^* \subset \left(\overline{S}\right)^*$.
> >
> > </div>
> >
> > </div>
>
> </div>
>
> </div>

> [!EXAMPLE]
>
> ### Example
>
> <div>
>
> <div class="callout-example">
>
> Prove that $\left( \mathbf{conv}(S) \right)^* = S^*$.
>
> > [!SOLUTION]
> >
> > ### Solution
> >
> > <div>
> >
> > <div class="callout-solution" collapse="true">
> >
> > - $S \subset \mathbf{conv}(S) \to \left( \mathbf{conv}(S) \right)^* \subset S^*$.
> >
> > - Let $p \in S^*$, $x_0 \in \mathbf{conv}(S)$, i.e.,
> >   $x_0 = \sum\limits_{i=1}^k\theta_i x_i \mid x_i \in S, \sum\limits_{i=1}^k\theta_i = 1, \theta_i \ge 0$.
> >
> >   So
> >   $p^T x_0 = \sum\limits_{i=1}^k\theta_i p^Tx_i \ge \sum\limits_{i=1}^k\theta_i (-1) = 1 \cdot (-1) = -1$.
> >   So $p \in \left( \mathbf{conv}(S) \right)^*$, hence
> >   $S^* \subset \left( \mathbf{conv}(S) \right)^*$.
> >
> > </div>
> >
> > </div>
>
> </div>
>
> </div>

> [!EXAMPLE]
>
> ### Example
>
> <div>
>
> <div class="callout-example">
>
> Prove that if $B(0,r)$ is a ball of radius $r$ by some norm centered
> at zero, then $\left( B(0,r) \right)^* = B(0,1/r)$.
>
> > [!SOLUTION]
> >
> > ### Solution
> >
> > <div>
> >
> > <div class="callout-solution" collapse="true">
> >
> > - Let $B(0,r) = X, B(0,1/r) = Y$. Take the normal vector
> >   $p \in X^*$, then for any $x \in X: p^Tx \ge -1$.
> >
> > - From all points of the ball $X$, take such a point $x \in X$ that
> >   its scalar product of $p$: $p^Tx$ is minimal, then this is the
> >   point $x = -\frac{p}{\|p\|}r$.
> >
> >   $$
> >     p^T x = p^T \left(-\frac{p}{\|p\||}r \right) = -\|p\|r \ge -1
> >     $$
> >
> >   $$
> >     \|p\| \le \frac{1}{r} \in Y
> >     $$
> >
> >   So $X^* \subset Y$.
> >
> > - Now let $p \in Y$. We need to show that $p \in X^*$, i.e.,
> >   $\langle p, x\rangle \geq -1$. It’s enough to apply the
> >   Cauchy-Bunyakovsky inequality:
> >
> >   $$
> >     \|\langle p, x\rangle\| \leq \|p\| \|x\| \leq \dfrac{1}{r} \cdot r = 1
> >     $$
> >
> >   The latter comes from the fact that $p \in B(0,1/r)$ and
> >   $x \in B(0,r)$.
> >
> >   So $Y \subset X^*$.
> >
> > </div>
> >
> > </div>
>
> </div>
>
> </div>

### Dual cones

A conjugate cone to a cone $K$ is a set $K^*$ such that:

$$
K^* = \left\{ y \mid \langle x, y\rangle \ge 0 \quad \forall x \in K\right\}
$$

To show that this definition follows directly from the theorem above,
recall what a conjugate set is and what a cone $\forall \lambda > 0$ is.

$$
\{y \in \mathbb{R}^n \mid \langle y, x\rangle \ge -1 \;\; \forall x \in S\} \to \to \{\lambda y \in \mathbb{R}^n \mid \langle y, x\rangle \ge -\dfrac{1}{\lambda} \;\; \forall x\in S\}
$$

<div id="fig-conjugate_cone">

![](conjugate_cone.svg)

Figure 2: Illustration of dual cone

</div>

### Dual cones properties

- Let $K$ be a closed convex cone. Then $K^{**} = K$.

- For an arbitrary set $S \subseteq \mathbb{R}^n$ and a cone
  $K \subseteq \mathbb{R}^n$:

  $$
    \left( S + K \right)^* = S^* \cap K^*
    $$

- Let $K_1, \ldots, K_m$ be cones in $\mathbb{R}^n$, then:

  $$
    \left( \sum\limits_{i=1}^m K_i \right)^* = \bigcap\limits_{i=1}^m K_i^*
    $$

- Let $K_1, \ldots, K_m$ be cones in $\mathbb{R}^n$. Let also their
  intersection have an interior point, then:

  $$
    \left( \bigcap\limits_{i=1}^m K_i \right)^* = \sum\limits_{i=1}^m K_i^*
    $$

### Examples

> [!EXAMPLE]
>
> ### Example
>
> <div>
>
> <div class="callout-example">
>
> Find the conjugate cone for a monotone nonnegative cone:
>
> $$
> K = \left\{ x \in \mathbb{R}^n \mid x_1 \ge x_2 \ge \ldots \ge x_n \ge 0\right\}
> $$
>
> > [!SOLUTION]
> >
> > ### Solution
> >
> > <div>
> >
> > <div class="callout-solution" collapse="true">
> >
> > Note that:
> >
> > $$
> > \sum\limits_{i=1}^nx_iy_i = y_1 (x_1-x_2) + (y_1 + y_2)(x_2 - x_3) + \ldots + (y_1 + y_2 + \ldots + y_{n-1})(x_{n-1} - x_n) + (y_1 + \ldots + y_n)x_n
> > $$
> >
> > Since in the presented sum in each summand, the second multiplier in
> > each summand is non-negative, then:
> >
> > $$
> > y_1 \ge 0, \;\; y_1 + y_2 \ge 0, \;\;\ldots, \;\;\;y_1 + \ldots + y_n \ge 0
> > $$
> >
> > So
> > $K^* = \left\{ y \mid \sum\limits_{i=1}^k y_i \ge 0, k = \overline{1,n}\right\}$.
> >
> > </div>
> >
> > </div>
>
> </div>
>
> </div>

### Polyhedra

The set of solutions to a system of linear inequalities and equalities
is a polyhedron:

$$
Ax \preceq b, \;\;\; Cx = d
$$

Here $A \in \mathbb{R}^{m\times n}, C \in \mathbb{R}^{p \times n}$, and
the inequality is a piecewise inequality.

<div id="fig-polyhedra">

![](polyhedra.svg)

Figure 3: Polyhedra

</div>

> [!THEOREM]
>
> ### Theorem
>
> <div>
>
> <div class="callout-theorem">
>
> Let $x_1, \ldots, x_m \in \mathbb{R}^n$. Conjugate to a polyhedral
> set:
>
> $$
> S = \mathbf{conv}(x_1, \ldots, x_k) + \mathbf{cone}(x_{k+1}, \ldots, x_m) 
> $$
>
> is a polyhedron (polyhedron):
>
> $$
> S^* = \left\{ p \in \mathbb{R}^n \mid \langle p, x_i\rangle \ge -1, i = \overline{1,k} ; \langle p, x_i\rangle \ge 0, i = \overline{k+1,m} \right\}
> $$
>
> > [!PROOF]
> >
> > ### Proof
> >
> > <div>
> >
> > <div class="callout-proof" collapse="true">
> >
> > - Let $S = X, S^* = Y$. Take some $p \in X^*$, then
> >   $\langle p, x_i\rangle \ge -1, i = \overline{1,k}$. At the same
> >   time, for any $\theta > 0, i = \overline{k+1,m}$:
> >
> >   $$
> >     \langle p, x_i\rangle \ge -1 \to \langle p, \theta x_i\rangle \ge -1
> >     $$
> >
> >   $$
> >     \langle p, x_i\rangle \ge -\frac{1}{\theta} \to \langle p, x_i\rangle \geq 0. 
> >     $$
> >
> >   So $p \in Y \to X^* \subset Y$.
> >
> > - Suppose, on the other hand, that $p \in Y$. For any point
> >   $x \in X$:
> >
> >   $$
> >      x = \sum\limits_{i=1}^m\theta_i x_i \;\;\;\;\;\;\; \sum\limits_{i=1}^k\theta_i = 1, \theta_i \ge 0
> >     $$
> >
> >   So:
> >
> >   $$
> >     \langle p, x\rangle = \sum\limits_{i=1}^m\theta_i \langle p, x_i\rangle = \sum\limits_{i=1}^k\theta_i \langle p, x_i\rangle + \sum\limits_{i=k+1}^m\theta_i \langle p, x_i\rangle \ge \sum\limits_{i=1}^k\theta_i (-1) + \sum\limits_{i=1}^k\theta_i \cdot 0 = -1.
> >     $$
> >
> >   So $p \in X^* \to Y \subset X^*$.
> >
> > </div>
> >
> > </div>
>
> </div>
>
> </div>

> [!EXAMPLE]
>
> ### Example
>
> <div>
>
> <div class="callout-example">
>
> Find and represent the set conjugate to a polyhedral cone in the
> plane:
>
> $$
> S = \mathbf{cone} \left\{ (-3,1), (2,3), (4,5)\right\}
> $$
>
> > [!SOLUTION]
> >
> > ### Solution
> >
> > <div>
> >
> > <div class="callout-solution" collapse="true">
> >
> > Using the theorem above:
> >
> > $$
> > S^* = \left\{ -3p_1 + p_2 \ge 0, 2p_1 + 3p_2 \ge 0, 4p_1+5p_2 \ge 0 \right\} 
> > $$
> >
> > </div>
> >
> > </div>
>
> </div>
>
> </div>

#### Farkas’ Lemma

Let $A \in \mathbb{R}^{m\times n}, b \in \mathbb{R}^m$. Then one and
only one of the following two systems has a solution:

$$
1) \; Ax = b, x \ge 0
$$

$$
2) \; p^\top A \ge 0, \langle p,b\rangle < 0.
$$

$Ax = b$ when $x \geq 0$ means that $b$ lies in a cone stretched over
the columns of the matrix $A$.

$pA \geq 0, \; \langle p, b \rangle < 0$ means that there exists a
separating hyperplane between the vector $b$ and the cone of columns of
the matrix $A$.

##### Corollary:

Let $A \in \mathbb{R}^{m\times n}, b \in \mathbb{R}^m$. Then one and
only one of the following two systems has a solution:

$$
1) Ax \leq b
$$

$$
2) p^\top A = 0, \langle p,b\rangle < 0, p \ge 0.
$$

If in the minimization linear programming problem, the budget set is
non-empty and the target function is bounded on it from below, then the
problem has a solution.
